WIP in inductives

pcuic/theories/PCUICInductives.v
@@ -1666,6 +1666,494 @@ Proof.
       rewrite it_mkProd_or_LetIn_app /= //.
 Qed.
 
+Lemma wf_local_expand_lets {cf} {Σ} {wfΣ : wf Σ} {Γ Δ Γ'} : 
+  wf_local Σ (Γ ,,, Δ ,,, Γ') ->
+  wf_local Σ (Γ ,,, smash_context [] Δ ,,, expand_lets_ctx Δ Γ').
+Proof.
+  intros hwf.
+  rewrite /expand_lets_ctx /expand_lets_k_ctx.
+  destruct (wf_local_app_inv hwf) as [wfΓΔ _].
+  rewrite -app_context_assoc in hwf.
+  eapply (weakening_wf_local (Γ'' := smash_context [] Δ)) in hwf.
+  len in hwf. simpl in hwf. simpl.
+  2:{ eapply wf_local_smash_end; pcuic. }
+  rewrite lift_context_app app_context_assoc Nat.add_0_r in hwf.
+  eapply substitution_wf_local in hwf; tea.
+  now eapply PCUICContexts.subslet_extended_subst.
+Qed.
+
+Lemma to_extended_list_k_map_lift:
+  forall (n k : nat) (c : context), 
+  to_extended_list_k c k = map (lift n (#|c| + k)) (to_extended_list_k c k).
+Proof.
+  intros n k c.
+  pose proof (to_extended_list_k_spec c k). unf_term.
+  symmetry. solve_all.
+  destruct H as [x' [-> Hx]]. simpl.
+  destruct (leb_spec_Set (#|c| + k) x').
+  - f_equal. lia.
+  - reflexivity.
+Qed.
+
+Lemma all_rels_smash Γ n k : 
+  assumption_context Γ ->
+  all_rels Γ n k = List.rev (to_extended_list_k Γ n).
+Proof.
+  induction 1 in n, k |- *; cbn; auto.
+  rewrite reln_acc rev_app_distr /=.
+  f_equal. rewrite IHassumption_context Nat.add_1_r //.
+Qed.
+
+Lemma to_extended_list_k_expand_lets Γ n Δ i : 
+  to_extended_list_k (expand_lets_k_ctx Γ n Δ) i = to_extended_list_k Δ i.
+Proof.
+  rewrite /expand_lets_k_ctx.
+  now rewrite to_extended_list_k_subst to_extended_list_k_lift_context.
+Qed.
+
+
+From MetaCoq.PCUIC Require Import PCUICRename.
+
+Lemma extended_subst_lift_context n (Γ : context) (k k' : nat) :
+  extended_subst (lift_context n k Γ) k' =
+  map (lift n (k + context_assumptions Γ + k')) (extended_subst Γ k').
+Proof.
+  pose proof (PCUICRename.rename_extended_subst).
+  rewrite -rename_context_lift_context.
+  rewrite lift_extended_subst -H.
+  rewrite (lift_extended_subst _ k').
+  rewrite !map_map_compose. apply map_ext => t.
+  rewrite shiftn_lift_renaming; sigma.
+  apply inst_ext.
+  rewrite - !Upn_Upn (Nat.add_comm _ k') !Upn_Upn shiftn_Upn - !Upn_Upn.
+  move=> i; lia_f_equal.
+Qed.
+
+Lemma subst_context_lift_context (n : nat) (Γ Δ : context) :
+  subst_context (extended_subst (lift_context n 0 Γ) 0) 0 (lift_context n (#|Γ| + context_assumptions Γ) Δ) =
+  lift_context n (context_assumptions Γ) (subst_context (extended_subst Γ 0) 0 Δ).
+Proof.
+  rewrite {1}extended_subst_lift_context /= Nat.add_0_r.
+  now rewrite distr_lift_subst_context; len.
+Qed.
+Lemma lift_context_lift_context n k k' Γ : 
+  lift_context n (k + k') (lift_context k' k Γ) = lift_context (n + k') k Γ.
+Proof.
+  rewrite - !rename_context_lift_context.
+  rewrite /PCUICRename.rename_context fold_context_k_compose.
+  apply fold_context_k_ext => i x.
+  rewrite !rename_inst !shiftn_lift_renaming !ren_lift_renaming.
+  sigma. apply inst_ext.
+  now rewrite Upn_compose Upn_compose shiftn_Upn shiftk_compose.
+Qed.
+
+Lemma lift_context_subst_context_let_expand n s Γ Δ : 
+  #|s| = context_assumptions Γ ->
+  lift_context n 0 (subst_context_let_expand s Γ Δ) =
+  subst_context_let_expand (map (lift0 n) s) (lift_context n 0 Γ) (lift_context n #|Γ| Δ).
+Proof.
+  intros hlen.
+  rewrite /subst_context_let_expand.
+  rewrite distr_lift_subst_context. f_equal.
+  rewrite Nat.add_0_r hlen.
+  rewrite /expand_lets_ctx /expand_lets_k_ctx /=; autorewrite with len.
+  rewrite -lift_context_add Nat.add_comm lift_context_add.
+  rewrite -subst_context_lift_context.
+  rewrite -lift_context_add.
+  now rewrite lift_context_lift_context.
+Qed.
+
+
+Lemma expand_lets_lift n k Γ t : 
+  expand_lets (lift_context n k Γ) (lift n (#|Γ| + k) t) =
+  lift n (k + context_assumptions Γ) (expand_lets Γ t).
+Proof.
+  rewrite /expand_lets /expand_lets_k /=.
+  rewrite extended_subst_lift_context Nat.add_0_r.
+  epose proof (distr_lift_subst_rec _ _ _ 0 (k + context_assumptions Γ)).
+  len. rewrite permute_lift. lia. rewrite !Nat.add_assoc /= in H.
+  relativize #|Γ|. erewrite <- H. 2:now len.
+  now len.
+Qed.
+
+Lemma expand_lets_ctx_lift n k' Γ Δ : 
+  k' = #|Γ| ->
+  expand_lets_ctx (lift_context n 0 Γ) (lift_context n k' Δ) =
+  lift_context n (context_assumptions Γ) (expand_lets_ctx Γ Δ).
+Proof.
+  intros ->.
+  rewrite /expand_lets_ctx /expand_lets_k_ctx /=.
+  len.
+  rewrite distr_lift_subst_context. len.
+  rewrite -lift_context_add Nat.add_comm.
+  rewrite lift_context_lift_context.
+  now rewrite extended_subst_lift_context. 
+Qed.
+
+Lemma lift_context_expand_lets_ctx n Γ Δ : 
+  lift_context n 0 (expand_lets_ctx Γ Δ) =
+  expand_lets_k_ctx Γ n (lift_context n 0 Δ).
+Proof.
+  rewrite /expand_lets_ctx /expand_lets_k_ctx.
+  rewrite lift_context_subst_context. f_equal.
+  rewrite - !rename_context_lift_context /rename_context !fold_context_k_compose.
+  apply fold_context_k_ext => i t.
+  rewrite !shiftn_lift_renaming; sigma.
+  apply inst_ext. now rewrite !Upn_compose shiftn_Upn.
+Qed.
+
+Lemma typing_expand_lets_gen {cf} {Σ} {wfΣ : wf Σ} {Γ Δ Γ' t T} : 
+  Σ ;;; Γ ,,, Δ ,,, Γ' |- t : T -> 
+  Σ ;;; Γ ,,, smash_context [] Δ ,,, expand_lets_ctx Δ Γ' |- 
+    expand_lets_k Δ #|Γ'| t : expand_lets_k Δ #|Γ'| T. 
+Proof.
+  intros Ht.
+  rewrite /expand_lets /expand_lets_k.
+  pose proof (typing_wf_local Ht).
+  rewrite -app_context_assoc in Ht.
+  eapply (weakening_typing (Γ'' := smash_context [] Δ)) in Ht.
+  len in Ht. simpl in Ht. simpl.
+  2:{ eapply wf_local_smash_end; pcuic. now apply wf_local_app_inv in X. }
+  rewrite lift_context_app app_context_assoc Nat.add_0_r in Ht.
+  eapply substitution in Ht; tea.
+  2:{ eapply PCUICContexts.subslet_extended_subst. now apply wf_local_app_inv in X. }
+  now len in Ht.
+Qed.
+
+Lemma expand_lets_k_subst_comm Δ k s T : 
+  expand_lets_k Δ k (subst0 s T) = 
+  subst0 (map (expand_lets_k Δ k) s) (expand_lets_k Δ (#|s| + k) T).
+Proof.
+  rewrite /expand_lets_k.
+  now rewrite distr_lift_subst distr_subst Nat.add_assoc map_map_compose; len.
+Qed.
+
+Definition subst_let_expand_k args Δ k T := 
+  (subst args k (expand_lets_k Δ k T)).
+
+Lemma map_subst_let_expand_k args Δ k l : 
+  map (subst args k) (map (expand_lets_k Δ k) l) =
+  map (subst_let_expand_k args Δ k) l.
+Proof.
+  now rewrite map_map_compose.
+Qed.
+
+Lemma subst_let_expand_k_0 s Γ :
+  subst_let_expand_k s Γ 0 =1 subst_let_expand s Γ.
+Proof. reflexivity. Qed.
+
+
+
+Lemma subst_let_expand_it_mkProd_or_LetIn s Γ Δ T : 
+  subst_let_expand s Γ (it_mkProd_or_LetIn Δ T) =
+  it_mkProd_or_LetIn (subst_context_let_expand s Γ Δ) (subst_let_expand_k s Γ #|Δ| T). 
+Proof.
+  rewrite /subst_let_expand /expand_lets.
+  rewrite expand_lets_it_mkProd_or_LetIn /= subst_it_mkProd_or_LetIn /=.
+  len. 
+Qed.
+
+Lemma subst_let_expand_k_mkApps s Γ k f args :
+  subst_let_expand_k s Γ k (mkApps f args) = 
+  mkApps (subst_let_expand_k s Γ k f) (map (subst_let_expand_k s Γ k) args).
+Proof.
+  rewrite /subst_let_expand_k.
+  now rewrite expand_lets_k_mkApps subst_mkApps map_map_compose.
+Qed.
+
+Lemma expand_lets_k_to_extended_list_k Γ k : 
+  map (expand_lets_k Γ k) (to_extended_list_k Γ k) = to_extended_list_k (smash_context [] Γ) k.
+Proof.
+  rewrite /expand_lets_k -map_map_compose.
+  rewrite -extended_subst_to_extended_list_k.
+  f_equal. now rewrite Nat.add_comm -to_extended_list_k_map_lift.
+Qed.
+
+Lemma map_subst_let_expand_k_to_extended_list_lift {cf} {Σ s Γ Δ k} :
+  spine_subst Σ Γ s (List.rev s) (smash_context [] Δ) ->
+  map (subst_let_expand_k (List.rev s) Δ k) (to_extended_list_k Δ k) = map (lift0 k) s.
+Proof.
+  intros sp.
+  eapply spine_subst_subst_to_extended_list_k in sp.
+  rewrite /subst_let_expand_k.
+  rewrite -map_map_compose.
+  rewrite expand_lets_k_to_extended_list_k.
+  rewrite -{2}(Nat.add_0_r k).
+  rewrite PCUICLiftSubst.lift_to_extended_list_k -{2}sp !map_map_compose.
+  apply map_ext. intros x.
+  now rewrite commut_lift_subst_rec.
+Qed.
+
+Lemma map_subst_let_expand_to_extended_list {cf} {Σ s Γ Δ} :
+  spine_subst Σ Γ s (List.rev s) (smash_context [] Δ) ->
+  map (subst_let_expand (List.rev s) Δ) (to_extended_list Δ) = s.
+Proof.
+  intros sp.
+  specialize (map_subst_let_expand_k_to_extended_list_lift (k:=0) sp).
+  now rewrite map_lift0.
+Qed.
+
+Lemma map_subst_let_expand_lift {s Γ k s'} :
+  #|s| = context_assumptions Γ -> k = #|Γ| ->
+  map (subst_let_expand s Γ) (map (lift0 k) s') = s'.
+Proof.
+  intros hs hlen.
+  rewrite /subst_let_expand map_map_compose.
+  rewrite -{2}(map_id s'). apply map_ext => t.
+  rewrite /expand_lets /expand_lets_k /=.
+  sigma. rewrite hlen.
+  rewrite -subst_compose_assoc.
+  rewrite shiftn_Upn. sigma.
+  rewrite subst_consn_shiftn. 2:now len.
+  now rewrite subst_consn_shiftn; sigma.
+Qed.
+
+Lemma subst_let_expand_k_lift s Γ n k t : 
+  n = #|Γ| -> #|s| = context_assumptions Γ ->
+  subst_let_expand_k s Γ 0 (lift0 (n + k) t) = lift0 k t. 
+Proof.
+  intros.
+  rewrite -(simpl_lift _ _ _ _ 0); try lia.
+  rewrite subst_let_expand_k_0.
+  rewrite subst_let_expand_lift_id //.
+Qed.
+
+Lemma expand_lets_k_0 Γ t : expand_lets_k Γ 0 t = expand_lets Γ t.
+Proof. reflexivity. Qed.
+
+
+Lemma smash_context_app_expand_acc Γ Δ : 
+  smash_context [] Γ ,,, expand_lets_ctx Γ Δ = 
+  smash_context Δ Γ.
+Proof.
+  rewrite (smash_context_acc Γ Δ). reflexivity.
+Qed.
+
+Lemma expand_lets_ctx_app Δ Γ Γ' : 
+  expand_lets_ctx Δ (Γ ,,, Γ') = expand_lets_ctx Δ Γ ,,, expand_lets_k_ctx Δ #|Γ| Γ'.
+Proof.
+  rewrite /expand_lets_ctx /expand_lets_k_ctx lift_context_app subst_context_app; len => //.
+Qed.
+
+Lemma lift_context_subst Γ p s n k : 
+  context_subst Γ p s -> 
+  context_subst (lift_context n k Γ) (map (lift n k) p) (map (lift n k) s).
+Proof.
+  induction 1 in |- *; try constructor.
+  rewrite lift_context_snoc map_app /=; constructor; auto.
+  rewrite lift_context_snoc /= /lift_decl /map_decl /=.
+  rewrite (context_subst_length X).
+  rewrite distr_lift_subst.
+  now constructor.
+Qed.
+
+Lemma subst_context_subst Γ p s sub k : 
+  context_subst Γ p s -> 
+  context_subst (subst_context sub k Γ) (map (subst sub k) p) (map (subst sub k) s).
+Proof.
+  induction 1 in |- *; try constructor.
+  rewrite subst_context_snoc map_app /=; constructor; auto.
+  rewrite subst_context_snoc /= /subst_decl /map_decl /=.
+  rewrite (context_subst_length X).
+  rewrite distr_subst.
+  now constructor.
+Qed.
+
+Lemma subslet_smash_context {cf} {Σ} {wfΣ : wf Σ} {Γ Δ Γ' Δ' s} :
+  subslet Σ (Γ ,,, Δ ,,, Γ') s Δ' ->
+  subslet Σ (Γ ,,, smash_context [] Δ ,,, expand_lets_ctx Δ Γ')
+    (map (expand_lets_k Δ #|Γ'|) s) (expand_lets_k_ctx Δ #|Γ'| Δ').
+Proof.
+  induction 1.
+  * simpl. constructor.
+  * simpl. rewrite /expand_lets_k_ctx lift_context_snoc subst_context_snoc.
+    constructor. apply IHX. len.
+    rewrite Nat.add_assoc. fold (expand_lets_k Δ (#|Δ0| + #|Γ'|) T).
+    eapply typing_expand_lets_gen in t0.
+    rewrite expand_lets_k_subst_comm in t0.
+    now rewrite -(subslet_length X).
+  * simpl. rewrite /expand_lets_k_ctx lift_context_snoc subst_context_snoc.
+    len. rewrite /subst_decl /lift_decl /map_decl /=.
+    eapply subslet_def. apply IHX. len.
+    rewrite !Nat.add_assoc. 
+    fold (expand_lets_k Δ (#|Δ0| + #|Γ'|) t).
+    fold (expand_lets_k Δ (#|Δ0| + #|Γ'|) T).
+    eapply typing_expand_lets_gen in t0.
+    rewrite !expand_lets_k_subst_comm in t0.
+    now rewrite -(subslet_length X).
+    now rewrite expand_lets_k_subst_comm -(subslet_length X) Nat.add_assoc.
+Qed.
+
+Lemma spine_subst_expand_lets {cf Σ} {wfΣ : wf Σ} {Γ Δ Γ'} {inst s Δ'} : 
+  spine_subst Σ (Γ ,,, Δ ,,, Γ') inst s Δ' ->
+  spine_subst Σ (Γ ,,, smash_context [] Δ ,,, expand_lets_ctx Δ Γ') 
+    (map (expand_lets_k Δ #|Γ'|) inst) (map (expand_lets_k Δ #|Γ'|) s)
+    (expand_lets_k_ctx Δ #|Γ'| Δ').
+Proof.
+  intros [].
+  split.
+  * rewrite -app_context_assoc.
+    rewrite smash_context_app_expand_acc.
+    eapply wf_local_app_inv in spine_dom_wf as [wfΔ wfΓ'].
+    eapply wf_local_app. now apply wf_local_app_inv in wfΔ.
+    eapply wf_local_rel_smash_context_gen; tea.
+  * eapply wf_local_app_inv in spine_codom_wf as [wfΔ wfΓ'].
+    rewrite - !app_context_assoc -expand_lets_ctx_app.
+    apply wf_local_app_inv in wfΔ as [].
+    eapply wf_local_app. 
+    now apply wf_local_app_inv in a as [].
+    rewrite smash_context_app_expand_acc.
+    apply wf_local_rel_smash_context_gen; tea.
+    eapply wf_local_rel_app; tea.
+  * rewrite /expand_lets_k_ctx /expand_lets_k -map_map_compose -[map (fun t => _) s]map_map_compose.
+    eapply subst_context_subst.
+    now eapply lift_context_subst.
+  * now eapply subslet_smash_context.
+Qed.
+
+(* We show that the derived predicate of a case is always well-typed, for *any*
+  instance of the parameters (not just the ones from a well-formed predicate). *)
+Lemma wf_ind_predicate {cf : checker_flags} {Σ : global_env_ext} {wfΣ : wf Σ} {Γ} {ci : case_info}
+  {mdecl idecl} u :
+  wf_local Σ Γ ->
+  declared_inductive Σ ci mdecl idecl ->
+  consistent_instance_ext Σ (ind_universes mdecl) u ->
+  wf_local Σ (Γ ,,, smash_context [] (ind_params mdecl)@[u] ,,, (ind_predicate_context ci mdecl idecl)@[u]).
+Proof.
+  move=> wfΓ isdecl cu.
+  rewrite /pre_case_predicate_context_gen /inst_case_context /ind_predicate_context /=.
+  set (iass := {| decl_name := _ |}).
+  cbn.
+  rewrite [subst_instance_context _ _]subst_instance_expand_lets_ctx.
+  unshelve epose proof (on_inductive_inst isdecl _ _ _ cu); tea.
+  rewrite -/(subst_context_let_expand _ _ _).
+  rewrite subst_instance_app_ctx in X.
+  destruct X as [s Hs]. red in Hs.
+  eapply type_it_mkProd_or_LetIn_inv in Hs as (idxs & inds & [sortsidx sortind leq]).
+  set (idxctx := smash_context [] (ind_params mdecl)@[u] ,,, expand_lets_ctx (ind_params mdecl)@[u] (ind_indices idecl)@[u]) in *.
+  have tyass : Σ ;;; Γ ,,, idxctx |- (decl_type iass)@[u] : tSort (ind_sort idecl)@[u].
+  { pose proof (on_inductive_sort_inst isdecl _ cu).
+    rewrite /iass /=.
+    have wfidxctx : wf_local Σ (Γ ,,, idxctx).
+    { rewrite /idxctx. rewrite app_context_assoc.
+      apply wf_local_expand_lets. rewrite -app_context_assoc.
+      eapply weaken_wf_local => //. rewrite -subst_instance_app_ctx.
+      eapply on_minductive_wf_params_indices_inst; tea.
+    }
+    rewrite subst_instance_mkApps /=; cbn.
+    erewrite subst_instance_id_mdecl; tea.
+    eapply pre_type_mkApps_arity. econstructor; tea.
+    eapply declared_inductive_valid_type; tea.
+    pose proof (on_declared_inductive isdecl) as [onmind oib].
+    rewrite oib.(ind_arity_eq) !subst_instance_it_mkProd_or_LetIn 
+      subst_instance_to_extended_list subst_instance_app_ctx
+      subst_instance_smash.
+    (* rewrite -it_mkProd_or_LetIn_app. *)
+    rewrite /to_extended_list to_extended_list_k_app.
+    rewrite Nat.add_0_r. len.
+    eapply arity_spine_it_mkProd_or_LetIn_smash.
+    - rewrite -(closed_ctx_lift #|ind_indices idecl| 0 (ind_params mdecl)@[u]).
+      { rewrite closedn_subst_instance_context.
+        eapply (declared_inductive_closed_params isdecl). }
+      rewrite (smash_context_lift []).
+      rewrite /idxctx app_context_assoc.
+      rewrite to_extended_list_k_lift_context.
+      replace #|ind_indices idecl| with (#|ind_indices idecl| + 0) by lia.
+      rewrite PCUICLiftSubst.lift_to_extended_list_k Nat.add_0_r.
+      rewrite -map_rev.
+      relativize #|ind_indices idecl|.
+      eapply subslet_lift; tea => //.
+      now rewrite -app_context_assoc. 2:len.
+      epose proof (spine_subst_to_extended_list_k (Γ := Γ) (Δ := smash_context [] (ind_params mdecl)@[u])); tea.
+      forward X.
+      { apply wf_local_smash_end, weaken_wf_local => //. eapply on_minductive_wf_params; tea. eapply isdecl. }
+      destruct X. len in inst_subslet.
+      rewrite PCUICClosed.closed_ctx_lift in inst_subslet => //.
+      apply closedn_smash_context.
+      rewrite closedn_subst_instance_context.
+      apply (declared_inductive_closed_params isdecl).
+      rewrite all_rels_smash in inst_subslet.
+      { apply smash_context_assumption_context. constructor. }
+      apply inst_subslet.
+    - rewrite subst_let_expand_it_mkProd_or_LetIn /=.
+      eapply arity_spine_it_mkProd_or_LetIn_Sort => //. reflexivity.
+      rewrite /subst_context_let_expand.
+      rewrite -expand_lets_k_ctx_subst_id'. admit. admit.
+      rewrite /idxctx app_context_assoc.
+      relativize #|ind_indices idecl|.
+      relativize (to_extended_list_k _ _).
+      eapply spine_subst_expand_lets. 3:len.
+      rewrite -subst_context_map_subst_expand_lets. len.
+      rewrite map_subst_extended_subst.
+      
+
+      rewrite -expand_lets_ctx_o_lets.
+      2:{ rewrite /expand_lets_ctx.
+          rewrite subst_instance_expand_lets_ctx.
+          rewrite to_extended_list_k_expand_lets. }
+      rewrite -subst_context_map_subst_expand_lets. len.
+
+      relativize (subst_context_let_expand _ _ _).
+      rewrite /idxctx. rewrite app_context_assoc.
+      rewrite subst_instance_expand_lets_ctx.
+      eapply spine_subst_to_extended_list_k.
+      now rewrite -app_context_assoc.
+      len.
+      rewrite /subst_context_let_expand.
+
+      rewrite /expand_lets_ctx.
+      rewrite /expand_lets_k_ctx. len.
+      rewrite lift_context_expand_lets_ctx.
+      rewrite PCUICLiftSubst.lift_to_extended_list_k. Nat.add_0_r.
+      rewrite subst_context_expand_lets_k
+
+
+      rewrite distr_lift_subst_context.
+      rewrite PCUICClosed.closed_ctx_lift //.
+      pose proof (PCUICContextSubst.context_subst_length2 sp).
+      rewrite context_assumptions_smash_context /= in H0. len in H0. len.
+      rewrite H0.
+      relativize (context_assumptions _).
+      eapply (PCUICClosed.closedn_ctx_expand_lets 0); len.
+      rewrite closedn_subst_instance_context.
+      apply (declared_inductive_closed_params isdecl).
+      2:len.
+      epose proof (declared_inductive_closed_pars_indices isdecl).
+      rewrite closedn_ctx_app in H1.
+      rewrite closedn_subst_instance_context.
+      move/andP: H1 => [] //.
+      f_equal. f_equal.
+      erewrite subst_to_extended_list_k => //.
+      rewrite /to_extended_list_k.
+
+      rewrite [reln [] _ _]to_extended_list_subst_context_let_expand.
+      apply PCUICLiftSubst.map_subst_instance_to_extended_list_k.
+      rewrite subst_context_let_expand_length subst_instance_length.
+      rewrite /subst_context_let_expand.
+      rewrite distr_lift_subst_context map_rev.
+      pose proof (PCUICContextSubst.context_subst_length2 sp).
+      rewrite context_assumptions_smash_context /= in H0. len in H0. len.
+      rewrite H0.
+      relativize (context_assumptions _).
+      eapply (PCUICClosed.closedn_ctx_expand_lets 0); len.
+    2:len.
+    epose proof (declared_inductive_closed_pars_indices isdecl).
+    rewrite closedn_ctx_app in H1.
+    rewrite closedn_subst_instance_context.
+    move/andP: H1 => [] //.
+    f_equal. f_equal.
+    erewrite subst_to_extended_list_k => //.
+    eapply make_context_subst_spec_inv. rewrite List.rev_involutive. cbn. apply sp. }
+  set (sdecl := subst_decl _ _ _).
+  rewrite -(it_mkProd_or_LetIn_app [sdecl]).
+  eapply type_it_mkProd_or_LetIn_sorts; tea.
+  constructor => //.
+  constructor => //. simpl.
+  constructor => //.
+  now eapply sorts_local_ctx_wf_local; tea. red.
+  eexists; tea. 
+Qed.
+
 (* We show that the derived predicate of a case is always well-typed, for *any*
   instance of the parameters (not just the ones from a well-formed predicate). *)
 Lemma isType_case_predicate {cf : checker_flags} {Σ : global_env_ext} {wfΣ : wf Σ} {Γ} {ci : case_info}
